---
title: "Derivando ando"
author: "Se√±or Ejemplo"
date: "30/11/2020"
output: html_document
---

### Derivando a(x)=x^6-89*x^(-4) respecto de x

```{r}
a<-expression(x^6-89*x^(-4))
aprima<-D(a,"x")
aprima
```

### Derivando b(x)=y*x^4-5*z*x^2 respecto de x

```{r}
b<-expression(y*x^4-5*z*x^2)
bprimax<-D(b,"x")
bprimax
```

### Derivando b(x)=y*x^4-5*z*x^2 respecto de y

```{r}
b<-expression(y*x^4-5*z*x^2)
bprimay<-D(b,"y")
bprimay
```

### Derivando b(x)=y*x^4-5*z*x^2 respecto de z

```{r}
b<-expression(y*x^4-5*z*x^2)
bprimaz<-D(b,"z")
bprimaz
```